Reformulate rtcTs to sequences

BinaryRelations.v
@@ -8,72 +8,59 @@ Require Import Coq.Program.Equality.
 Require Import Tactics.General.
 Require Import Tactics.Construct.
 
+Require Export Coq.Relations.Relation_Definitions.
+Require Export Coq.Relations.Relation_Operators.
+
+
+(* Misc. definitions *)
+
 Definition is_serial {A} (R: relation A) := forall a, exists b, R a b.
 Definition serial A := {R: relation A | is_serial R}.
 
-(* Definition is_serialT {A} (R: relation A) := forall a, {b | R a b}. *)
-(* Definition serialT A := {R: relation A & is_serialT R}. *)
 Definition serial_witness {A} (R: relation A) := forall a, {b | R a b}.
 Definition serialT A := {R: relation A & serial_witness R}.
-
-Definition reachable {A} (R: relation A) (l: list A) (b: A) := 
-  exists a, In a l /\ clos_refl_trans_n1 A R a b.
-
-Definition is_serial_from {A} (R: relation A) s := forall s', 
-  clos_refl_trans A R s s' ->
-  exists s'', R s' s''.
-
-Definition serial_from_witness {A} (R: relation A) s := forall s',
-  clos_refl_trans A R s s' ->
-  {s''| R s' s''}.
-
-Inductive steps : nat -> forall {A}, relation A -> relation A :=
-  | steps_one   : forall {A} (R: relation A) x y,
-      R x y -> steps 1 R x y
-  | steps_multi : forall {A} n (R: relation A) x y z,
-      steps n R x y -> R y x -> steps (S n) R x z.
 
 Definition rel_singleton {A} (x y : A): relation A :=
   fun x' y' => x' = x /\ y' = y -> True.
 
-
 Definition relationT A := A -> A -> Type.
 
-Reserved Notation "R ^*" (at level 5, format "R ^*").
-Inductive rtcT {A} (R: relation A) x : A -> Type :=
-  | rtcT_refl :
-      R^* x x
-  | rtcT_step : forall y z,
-      R y z ->
-      R^* x y ->
-      R^* x z
-  where "R ^*" := (rtcT R).
 
-Definition rtcT_singleton {state} {R: relation state} {x y} (r: R x y)
-  : R^* x y :=
-  rtcT_step R x x y r (rtcT_refl R x).
+(* star definition *)
+(* A reflexive transitive closure *)
 
-(* Definition rtc_ind_struct
-  (A: Type) (R: relation A) x (P: forall x y, R^* x y -> Prop)
-  (p_refl: P x x (rtn1_refl A R x))
-  (p_step: forall y z (Ryz: R y z) (Rxy: R^* x y),
-    P x y Rxy -> P x z (rtn1_trans A R x y z Ryz Rxy)) :=
-  fix F z (Rxy: R^* x z) : P x z Rxy :=
-    match Rxy with
-    | rtn1_refl _ _ _ => p_refl
-    | rtn1_trans _ _ _ y z0 Ryz Rxy => p_step y z0 Ryz Rxy (F y Rxy)
-    end.
+Definition star {A} (R: relation A) : relation A := clos_refl_trans_n1 A R.
+Notation "R ^*" := (star R) (at level 5, format "R ^*").
+
+Definition is_serial_from {A} (R: relation A) a :=
+  forall b,
+    R^* a b ->
+    exists c, R b c.
+
+Definition serial_from_witness {A} (R: relation A) a :=
+  forall b,
+    R^* a b ->
+    {c| R b c}.
+
+
+(* seq definition *)
+(* A transparent sequence of relation steps.
+   It is in fact just a reflexive transitive closure, but as a Type instead of a Prop
  *)
-(* Definition rtc_ind_struct
-  (A: Type) (R: relation A) (P: forall x y, R^* x y -> Prop)
-  (p_refl: forall x, P x x (rtn1_refl A R x))
-  (p_step: forall x y z (Ryz: R y z) (Rxy: R^* x y),
-    P x y Rxy -> P x z (rtn1_trans A R x y z Ryz Rxy)) :=
-  fix F x z (Rxy: R^* x z) : P x z Rxy :=
-    match Rxy with
-    | rtn1_refl _ _ _ => p_refl x
-    | rtn1_trans _ _ _ y z0 Ryz Rxy => p_step x y z0 Ryz Rxy (F x y Rxy)
-    end. *)
+
+Reserved Notation "R #*" (at level 5, format "R #*").
+Inductive seq {A} (R: relation A) : relationT A :=
+  | seq_refl : forall x,
+      R#* x x
+  | seq_step : forall x y z,
+      R y z ->
+      R#* x y ->
+      R#* x z
+  where "R #*" := (seq R).
+
+Definition seq_singleton {A} {R: relation A} {x y} (r: R x y)
+  : R#* x y :=
+  seq_step R x x y r (seq_refl R x).
 
 Definition reflexiveT {A} (R: relationT A) := forall x, R x x.
 
@@ -86,61 +73,67 @@ Definition transitiveT {A} (R: relationT A) := forall x y z,
   R y z -> 
   R x z.
 
-Lemma rtcT_trans {A}: forall R: relation A,
-  transitiveT R^*.
+Lemma seq_trans {A}: forall R: relation A,
+  transitiveT R#*.
 Proof.
   intros R x y z Hxy Hyz.
   induction Hyz.
   - assumption.
-  - econstructor; eassumption.
+  - econstructor.
+    + eassumption.
+    + applyc IHHyz.
+      assumption.
 Defined.
 
-Lemma rtcT_step_rev {A}: forall (R: relation A) a b c,
+Lemma seq_step_rev {A}: forall (R: relation A) a b c,
   R a b ->
-  R^* b c ->
-  R^* a c.
+  R#* b c ->
+  R#* a c.
 Proof.
   intros R a b c Hab Hbc.
-  eapply rtcT_trans; [|eassumption].
+  eapply seq_trans; [|eassumption].
   econstructor.
   - eassumption.
   - constructor.
 Defined.
 
-Inductive in_rtcT {A} {R: relation A} {a}
-  : forall {a'}, A -> R^* a a' -> Prop :=
-  | in_rtcT_head_refl :
-      in_rtcT a (rtcT_refl R a)
-  | in_rtcT_head_step : forall x x' r p,
-      in_rtcT x' (rtcT_step R a x x' r p)
-  | in_rtcT_tail : forall x x' y r p,
-      in_rtcT y p ->
-      in_rtcT y (rtcT_step R a x x' r p).
+Inductive in_seq {A} {R: relation A} {a}
+  : forall {a'}, A -> R#* a a' -> Prop :=
+  | in_seq_head_refl :
+      in_seq a (seq_refl R a)
+  | in_seq_head_step : forall x x' r p,
+      in_seq x' (seq_step R a x x' r p)
+  | in_seq_tail : forall x x' y r p,
+      in_seq y p ->
+      in_seq y (seq_step R a x x' r p).
 
-(* indexed rtc *)
 
-Reserved Notation "R ^#" (at level 5, format "R ^#").
-Inductive rtcT_idx {A} (R: relation A) : nat -> A -> A -> Type :=
-  | rtcT_idx_refl : forall x,
-      R^#0 x x
-  | rtcT_idx_step : forall n x y z,
+(* nseq definition (indexed seq) *)
+
+Reserved Notation "R #" (at level 5, format "R #").
+Inductive nseq {A} (R: relation A) : nat -> relationT A :=
+  | nseq_refl : forall x,
+      R#0 x x
+  | nseq_step : forall n x y z,
       R y z ->
-      R^#n x y ->
-      R^#(S n) x z
-  where "R ^#" := (rtcT_idx R).
+      R#n x y ->
+      R#(S n) x z
+  where "R #" := (nseq R).
+Notation "R # n" := (nseq R n) (at level 5, format "R # n").
 
-Definition rtcT_idx_singleton {state} {R: relation state} {x y} (r: R x y)
-  : R^# 1 x y :=
-  rtcT_idx_step R 0 x x y r (rtcT_idx_refl R x).
 
-Theorem rtcT_idx_step_rev {state}: forall (R: relation state) n s s' x,
+Definition nseq_singleton {A} {R: relation A} {x y} (r: R x y)
+  : R#1 x y :=
+  nseq_step R 0 x x y r (nseq_refl R x).
+
+Theorem nseq_step_rev {A}: forall (R: relation A) n s s' x,
   R s s' ->
-  R^# n s' x ->
-  R^# (S n) s x.
+  R#n s' x ->
+  R#(S n) s x.
 Proof using.
   intros R n s s' x Hstep Hpath.
   induction Hpath.
-  - apply rtcT_idx_singleton.
+  - apply nseq_singleton.
     assumption.
   - econstructor.
     + eassumption.
@@ -148,37 +141,33 @@ Proof using.
       assumption.
 Defined.
 
-(* Definition rtc_idx_ind_struct
-  (A: Type) (R: relation A) (P: forall n x y, R^# n x y -> Prop)
-  (p_refl: forall x, P 0 x x (rtc_idx_refl R x))
-  (p_step: forall n x y z (Ryz: R y z) (Rxy: R^# n x y),
-    P n x y Rxy -> P (S n) x z (rtc_idx_step R n x y z Ryz Rxy)) :=
-  fix F n x z (Rxy: R^# n x z) : P n x z Rxy :=
-    match Rxy as Rxy0 in (_^# n0 x0 y0) return (P n0 x0 y0 Rxy0) with
-    | rtc_idx_refl _ x0 => p_refl x0
-    | rtc_idx_step _ n0 x0 y z0 Ryz Rxy => p_step n0 x0 y z0 Ryz Rxy (F n0 x0 y Rxy)
-    end. *)
+Lemma nseq_step__nseq_step_rev {X}:
+  forall (R: relation X) s x x' n,
+    R x x' ->
+    R#n s x ->
+    {s' &
+      R s s' &
+      R#n s' x'}.
+Proof using.
+  introv Rxx' Rsx.
+  revert x' Rxx'.
+  induction Rsx; intros.
+  - exists x'.
+    + assumption. 
+    + constructor.
+  - applyc IHRsx in r.
+    destruct exists r s'.
+    exists s'.
+    + assumption.
+    + econstructor; eassumption.
+Qed.
 
-(* Definition rtc_idx_ind_struct_fixed_origin
-  (A: Type) (R: relation A) x (P: forall n x y, R^# n x y -> Prop)
-  (p_refl: P 0 x x (rtc_idx_refl R x))
-  (p_step: forall n y z (Ryz: R y z) (Rxy: R^# n x y),
-    P n x y Rxy -> P (S n) x z (rtc_idx_step R n x y z Ryz Rxy)) :=
-  fix F n z (Rxy: R^# n x z) : P n x z Rxy :=
-    (* match Rxy as Rxy0 in (_^# n0 x0 y0) return (P n0 x0 y0 Rxy0) with *)
-    match Rxy with
-    | rtc_idx_refl _ x0 => p_refl
-    | rtc_idx_step _ n0 x0 y z0 Ryz Rxy => p_step n0 x0 y z0 Ryz Rxy (F n0 y Rxy)
-    end. *)
-
-(* (almost) transitivity *)
-Theorem rtcT_idx_combine {A}: forall n m (R: relation A) x y z,
-  R^# n x y ->
-  R^# m y z ->
-  R^# (n+m) x z.
+Theorem nseq_trans {A}: forall n m (R: relation A) x y z,
+  R#n x y ->
+  R#m y z ->
+  R#(n+m) x z.
 Proof using.
   intros n m R x y z Hxy Hyz; revert x Hxy.
-  (* induction Hyz using rtc_idx_ind_struct; intros. *)
   induction Hyz; intros.
   - rewrite PeanoNat.Nat.add_0_r.
     assumption.
@@ -189,9 +178,9 @@ Proof using.
       assumption.
 Defined.
 
-Theorem rtcT_idx_to_rtcT {A n} {R: relation A} {x y}:
-  R^# n x y ->
-  R^* x y.
+Theorem nseq_to_seq {A n} {R: relation A} {x y}:
+  R#n x y ->
+  R#* x y.
 Proof using.
   introv H.
   induction H.
@@ -199,77 +188,52 @@ Proof using.
   - econstructor; eassumption.
 Defined.
 
-Theorem rtcT_to_rtcT_idx {A} {R: relation A} {x y}:
-  R^* x y ->
-  {n & R^# n x y}.
+Theorem seq_to_nseq {A} {R: relation A} {x y}:
+  R#* x y ->
+  {n & R#n x y}.
 Proof using.
   introv H.
   induction H.
   - eexists. constructor.
-  - destruct exists IHrtcT n.
+  - destruct exists IHseq n.
     exists (S n).
     econstructor; eassumption.
 Defined.
 
-Inductive in_rtcT_idx_at {A} {R: relation A} {a}
-  : forall {n a'}, A -> nat -> R^# n a a' -> Prop :=
-  | in_rtcT_idx_at_head_refl :
-      in_rtcT_idx_at a 0 (rtcT_idx_refl R a)
-  | in_rtcT_idx_at_head_step : forall n x x' r p,
-      in_rtcT_idx_at x' n (rtcT_idx_step R n a x x' r p)
-  | in_rtcT_idx_at_tail : forall n m x x' y r p,
-      in_rtcT_idx_at y m p ->
-      in_rtcT_idx_at y m (rtcT_idx_step R n a x x' r p).
+Inductive in_nseq_at {A} {R: relation A} {a}
+  : forall {n a'}, A -> nat -> R#n a a' -> Prop :=
+  | in_nseq_at_head_refl :
+      in_nseq_at a 0 (nseq_refl R a)
+  | in_nseq_at_head_step : forall n x x' r p,
+      in_nseq_at x' (S n) (nseq_step R n a x x' r p)
+  | in_nseq_at_tail : forall n m x x' y r p,
+      in_nseq_at y m p ->
+      in_nseq_at y m (nseq_step R n a x x' r p).
 
-Inductive in_rtcT_idx {A} {R: relation A} {a}
-  : forall {n a'}, A -> R^# n a a' -> Prop :=
-  | in_rtcT_idx_head_refl :
-      in_rtcT_idx a (rtcT_idx_refl R a)
-  | in_rtcT_idx_head_step : forall n x x' r p,
-      in_rtcT_idx x' (rtcT_idx_step R n a x x' r p)
-  | in_rtcT_idx_tail : forall n x x' y r p,
-      in_rtcT_idx y p ->
-      in_rtcT_idx y (rtcT_idx_step R n a x x' r p).
+Inductive in_nseq {A} {R: relation A} {a}
+  : forall {n a'}, A -> R#n a a' -> Prop :=
+  | in_nseq_head_refl :
+      in_nseq a (nseq_refl R a)
+  | in_nseq_head_step : forall n x x' r p,
+      in_nseq x' (nseq_step R n a x x' r p)
+  | in_nseq_tail : forall n x x' y r p,
+      in_nseq y p ->
+      in_nseq y (nseq_step R n a x x' r p).
 
-Definition in_rtcT_idx_ind_struct
-  (A : Type) (R : relation A) (a : A)
-  (P : forall (n : nat) (a' a0 : A) (r : R^# n a a'),
-	   in_rtcT_idx a0 r -> Prop)
-  (f : P 0 a a (rtcT_idx_refl R a) in_rtcT_idx_head_refl)
-  (f0 : forall (n : nat) (x x' : A) (r : R x x') (p : R^# n a x),
-        P (S n) x' x' (rtcT_idx_step R n a x x' r p)
-          (in_rtcT_idx_head_step n x x' r p))
-  (f1 : forall (n : nat) (x x' y : A) (r : R x x') 
-          (p : R^# n a x) (i : in_rtcT_idx y p),
-        P n x y p i ->
-        P (S n) x' y (rtcT_idx_step R n a x x' r p)
-          (in_rtcT_idx_tail n x x' y r p i)) :=
-fix F
-  (n : nat) (a' y : A) (r : R^# n a a') (i : in_rtcT_idx y r) {struct i} :
-    P n a' y r i :=
-  match
-    i as i0 in (@in_rtcT_idx _ _ _ n0 a'0 y0 r0) return (P n0 a'0 y0 r0 i0)
-  with
-  | in_rtcT_idx_head_refl => f
-  | in_rtcT_idx_head_step n0 x x' r0 p => f0 n0 x x' r0 p
-  | in_rtcT_idx_tail n0 x x' y0 r0 p i0 =>
-      f1 n0 x x' y0 r0 p i0 (F n0 x y0 p i0)
-  end.
-
-Theorem in_rtcT_idx_at__in_rtcT_idx {A}:
-  forall (R: relation A) x a b n m (r: R^# n a b),
-    in_rtcT_idx_at x m r ->
-    in_rtcT_idx x r.
+Theorem in_nseq_at__in_nseq {A}:
+  forall (R: relation A) x a b n m (r: R#n a b),
+    in_nseq_at x m r ->
+    in_nseq x r.
 Proof using.
   introv H.
   induction H; constructor.
   assumption.
 Qed.
 
-Theorem in_rtcT_idx__in_rtcT_idx_at {A}:
-  forall (R: relation A) x a b n (r: R^# n a b),
-    in_rtcT_idx x r ->
-    exists m, m <= n /\ in_rtcT_idx_at x m r.
+Theorem in_nseq__in_nseq_at {A}:
+  forall (R: relation A) x a b n (r: R#n a b),
+    in_nseq x r ->
+    exists m, m <= n /\ in_nseq_at x m r.
 Proof using.
   introv H.
   induction H.
@@ -279,29 +243,34 @@ Proof using.
   - eexists.
     split; [|constructor].
     lia.
-  - destruct exists IHin_rtcT_idx m.
+  - destruct exists IHin_nseq m.
     exists m.
-    destruct IHin_rtcT_idx.
+    destruct IHin_nseq.
     split.
     + lia.
     + constructor.
       assumption.
 Qed. 
 
-Theorem in_rtcT__in_rtcT_idx {A}:
-  forall (R: relation A) x a b (r: R^* a b),
-    in_rtcT x r ->
-    exists n (r': R^# n a b), in_rtcT_idx x r'.
+Theorem in_seq__in_nseq {A}:
+  forall (R: relation A) x a b (r: R#* a b),
+    in_seq x r ->
+    in_nseq x (projT2 (seq_to_nseq r)).
 Proof using.
-  introv.
-  dependent induction r; intros.
-  - repeat eexists. repeat constructor.
-Admitted.
+  intros R x a b r H.
+  induction H.
+  - simpl. constructor.
+  - simpl. break_let. simpl.
+    constructor.
+  - simpl. break_let. simpl in *.
+    constructor.
+    assumption.
+Qed.
 
-Theorem in_rtcT_idx__in_rtcT {A}:
-  forall (R: relation A) x n a b (r: R^# n a b),
-    in_rtcT_idx x r ->
-    in_rtcT x (rtcT_idx_to_rtcT r).
+Theorem in_nseq__in_seq {A}:
+  forall (R: relation A) x n a b (r: R#n a b),
+    in_nseq x r ->
+    in_seq x (nseq_to_seq r).
 Proof using.
   introv H.
   induction H. 
@@ -312,37 +281,95 @@ Proof using.
     assumption.
 Qed.
 
-Definition in_rtcT_idx_before {state} {R: relation state} {n s s'}
-  x i (r: R^# n s s') := 
-  exists j, j < i /\ in_rtcT_idx_at x i r.
+Definition in_nseq_before {state} {R: relation state} {n s s'}
+  x i (r: R#n s s') := 
+  exists j, j < i /\ in_nseq_at x j r.
 
-Theorem in_rtcT_idx__prefix {state}: 
-  forall (R: relation state) x y z n (Rxz: R^# n x z),
-    in_rtcT_idx y Rxz ~>
-    {m & m <= n & R^# m x y}.
-Proof using.
-  introv H.
-  dependent induction H.
-  - construct.
-    exists 0.
-    + reflexivity.
-    + constructor.
-  - construct.
-    exists (S n).
-    + reflexivity.
-    + econstructor; eassumption.
-  - uninhabit IHin_rtcT_idx.
-    destruct exists IHin_rtcT_idx m.
-    construct.
-    exists m.
-    + constructor. assumption.
-    + assumption.
+Inductive nseq_prefix {A} {R: relation A} {a}
+  : forall {n m b c}, R#n a b -> R#m a c -> Prop :=
+  | nseq_prefix_refl :
+      forall n b (Rab: R#n a b),
+        nseq_prefix Rab Rab
+  | nseq_prefix_step :
+      forall n b (Rab: R#n a b) m c (Rac: R#m a c) d (Rcd: R c d),
+        nseq_prefix Rab Rac ->
+        nseq_prefix Rab (nseq_step R m a c d Rcd Rac).
+
+Theorem nseq_prefix_trans {A}: forall {R: relation A} {nx ny nz a x y z},
+  forall (rx: R#nx a x) (ry: R#ny a y) (rz: R#nz a z),
+    nseq_prefix rx ry ->
+    nseq_prefix ry rz ->
+    nseq_prefix rx rz.
+Proof using. 
+  intros R nx nyz nz a x y z rx ry rz Hxy Hyz.
+  revert nx x rx Hxy.
+  induction Hyz; intros.
+  - assumption.
+  - constructor.
+    apply IHHyz.
+    assumption.
 Qed.
- 
-Theorem in_rtcT_idx__prefix' {state}: 
-  forall (R: relation state) x y z n (Rxz: R^# n x z),
-    in_rtcT_idx y Rxz ~>
-    R^* x y.
+
+Theorem in_nseq_at_prefix {A}:
+  forall (R: relation A) a nb b (Rab: R#nb a b) nc c (Rac: R#nc a c) x i,
+    nseq_prefix Rab Rac ->
+    in_nseq_at x i Rab ->
+    in_nseq_at x i Rac.
+Proof using.
+  intros R a nb b Rab nc c Rac x i Hprefix Hin.
+  induction Hprefix.
+  - assumption.
+  - constructor.
+    applyc IHHprefix.
+    assumption.
+Qed.
+
+Lemma nseq_prefix_before {A}:
+  forall (R: relation A) a nb b (Rab: R#nb a b) nc c (Rac: R#nc a c) x,
+    nseq_prefix Rab Rac ->
+    in_nseq x Rab ->
+    in_nseq_before x (S nb) Rac.
+Proof using.
+  intros R a nb b Rab nc c Rac x Hprefix Hin.
+  apply in_nseq__in_nseq_at in Hin.
+  destruct Hin as [m [Hlt Hin]].
+  exists m.
+  split.
+  - lia. 
+  - eapply in_nseq_at_prefix; eassumption.
+Qed.
+
+Theorem in_nseq_at__get_prefix {A}:
+  forall (R: relation A) x i n a b (r: R#n a b),
+    in_nseq_at x i r ->
+    exists r': R#i a x, nseq_prefix r' r.
+Proof using.
+  intros.
+  induction H.
+  - repeat eexists. constructor.
+  - repeat eexists. constructor.
+  - destruct exists IHin_nseq_at r'.
+    exists r'.
+    constructor.
+    assumption.
+Qed.
+
+Theorem in_nseq__get_prefix {A}: 
+  forall (R: relation A) x n a b (r: R#n a b),
+    in_nseq x r ->
+    exists m (r': R#m a x), nseq_prefix r' r.
+Proof using.
+  intros.
+  apply in_nseq__in_nseq_at in H as [i [_ H]].
+  exists i.
+  eapply in_nseq_at__get_prefix.
+  eassumption.
+Qed.
+
+Theorem in_nseq__get_prefix' {state}: 
+  forall (R: relation state) x y z n (Rxz: R#n x z),
+    in_nseq y Rxz ~>
+    R#* x y.
 Proof using.
   introv H.
   dependent induction H.
@@ -350,7 +377,7 @@ Proof using.
   - construct.
     econstructor.
     + eassumption.
-    + eapply rtcT_idx_to_rtcT.
+    + eapply nseq_to_seq.
       eassumption.
   - assumption.
 Qed.
