Classical.v
@@ -1,5 +1,7 @@
 Require Import Coq.Logic.Classical.
 
+Require Export Coq.Logic.Classical.
+
 Theorem destruct_impl : forall p q,
   ~p \/ p /\ q <-> (p -> q).
 Proof using.
@@ -10,3 +12,9 @@ Proof using.
     + intro H1. apply H.
   - destruct (classic p); auto.
 Qed.
+
+Tactic Notation "destruct" "classic" hyp(H) :=
+  destruct (classic H).
+
+Tactic Notation "destruct" "classic" ident(H) ":" uconstr(c) :=
+  destruct (classic c) as [H|H].
